restructure snapshot to not actually have a protocol on the y location

theories/logatom/snapshot/atomic_snapshot.v
@@ -11,16 +11,103 @@ Set Default Proof Using "Type".
 (** Specifying snapshots with histories
     Implementing atomic pair snapshot data structure from Sergey et al. (ESOP 2015) *)
 
+
+(*
+     newPair x y :=
+       (ref (ref (x, 0)), ref y)
+ *)
+Definition newPair : val :=
+  λ: "args",
+  let: "x" := Fst "args" in
+  let: "y" := Snd "args" in
+  (ref (ref ("x", #0)), ref "y").
+
+(*
+    writeY (xp, yp) y :=
+      yp <- y
+ *)
+Definition writeY : val :=
+  λ: "args",
+  let: "p" := Fst "args" in
+  Snd "p" <- Snd "args".
+
+(*
+    writeX (xp, yp) x :=
+      let xp1 = !xp in
+      let v   = (!xp1).2
+      let xp2 = ref (x, v + 1)
+      if CAS xp xp1 xp2
+        then ()
+        else writeX (xp, yp) x
+ *)
+Definition writeX : val :=
+  rec: "writeX" "args" :=
+    let: "p"    := Fst "args"             in
+    let: "x"    := Snd "args"             in
+    let: "xp"   := Fst "p"                in
+    let: "xp1"  := !"xp"                  in
+    let: "v"    := Snd (!"xp1")           in
+    let: "xp2"  := ref ("x", "v" + #1)    in
+    if: CAS "xp" "xp1" "xp2"
+    then #()
+    else "writeX" "args".
+
+(*
+    readX (xp, yp) :=
+      !!xp
+ *)
+Definition readX : val :=
+  λ: "p",
+  let: "xp" := Fst "p" in
+  !(!"xp").
+
+Definition readY : val :=
+  λ: "p",
+  let: "yp" := Snd "p" in
+  !"yp".
+
+(*
+    readPair l :=
+      let (x, v)  = readX l in
+      let y       = readY l in
+      let (_, v') = readX l in
+      if v = v'
+        then (x, y)
+        else readPair l
+ *)
+Definition readPair : val :=
+  rec: "readPair" "l" :=
+    let: "x"  := readX "l"  in
+    let: "y"  := readY "l"  in
+    let: "x'" := readX "l"  in
+    if: Snd "x" = Snd "x'"
+    then (Fst "x", Fst "y")
+    else  "readPair" "l".
+
+Definition readPair_proph : val :=
+  rec: "readPair" "l" :=
+    let: "xv1"    := readX "l"           in
+    let: "proph"  := NewProph            in
+    let: "y"      := readY "l"           in
+    let: "xv2"    := readX "l"           in
+    let: "v2"     := Snd "xv2"           in
+    let: "v_eq"   := Snd "xv1" = "v2"    in
+    resolve_proph: "proph" to: "v_eq" ;;
+    if: "v_eq"
+      then (Fst "xv1", "y")
+    else "readPair" "l".
+
+
 (** The CMRA & functor we need. *)
 
 Definition timestampUR := gmapUR Z $ agreeR valC.
 
 Class atomic_snapshotG Σ := AtomicSnapshotG {
-                                atomic_snapshot_stateG :> inG Σ $ authR $ optionUR $ exclR $ prodC valC valC;
+                                atomic_snapshot_stateG :> inG Σ $ authR $ optionUR $ exclR $ valC;
                                 atomic_snapshot_timestampG :> inG Σ $ authR $ timestampUR
 }.
 Definition atomic_snapshotΣ : gFunctors :=
-  #[GFunctor (authR $ optionUR $ exclR $ prodC valC valC); GFunctor (authR timestampUR)].
+  #[GFunctor (authR $ optionUR $ exclR $ valC); GFunctor (authR timestampUR)].
 
 Instance subG_atomic_snapshotΣ {Σ} : subG atomic_snapshotΣ Σ → atomic_snapshotG Σ.
 Proof. solve_inG. Qed.
@@ -29,120 +116,35 @@ Section atomic_snapshot.
 
   Context {Σ} `{!heapG Σ, !atomic_snapshotG Σ}.
 
-  (*
-     newPair x y :=
-       (ref (ref (x, 0)), ref y)
-   *)
-  Definition newPair : val :=
-    λ: "args",
-      let: "x" := Fst "args" in
-      let: "y" := Snd "args" in
-      (ref (ref ("x", #0)), ref "y").
-
-  (*
-    writeY (xp, yp) y :=
-      yp <- y
-  *)
-  Definition writeY : val :=
-    λ: "args",
-      let: "p" := Fst "args" in
-      Snd "p" <- Snd "args".
-
-  (*
-    writeX (xp, yp) x :=
-      let xp1 = !xp in
-      let v   = (!xp1).2
-      let xp2 = ref (x, v + 1)
-      if CAS xp xp1 xp2
-        then ()
-        else writeX (xp, yp) x
-  *)
-  Definition writeX : val :=
-    rec: "writeX" "args" :=
-      let: "p"    := Fst "args"             in
-      let: "x"    := Snd "args"             in
-      let: "xp"   := Fst "p"                in
-      let: "xp1"  := !"xp"                  in
-      let: "v"    := Snd (!"xp1")           in
-      let: "xp2"  := ref ("x", "v" + #1)    in
-      if: CAS "xp" "xp1" "xp2"
-        then #()
-      else "writeX" "args".
-
-  (*
-    readX (xp, yp) :=
-      !!xp
-   *)
-  Definition readX : val :=
-    λ: "p",
-      let: "xp" := Fst "p" in
-      !(!"xp").
-
-   Definition readY : val :=
-    λ: "p",
-      let: "yp" := Snd "p" in
-      !"yp".
-
-  (*
-    readPair l :=
-      let (x, v)  = readX l in
-      let y       = readY l in
-      let (_, v') = readX l in
-      if v = v'
-        then (x, y)
-        else readPair l
-  *)
-  Definition readPair : val :=
-    rec: "readPair" "l" :=
-      let: "x"  := readX "l"  in
-      let: "y"  := readY "l"  in
-      let: "x'" := readX "l"  in
-      if: Snd "x" = Snd "x'"
-        then (Fst "x", Fst "y")
-        else  "readPair" "l".
-
-  Definition readPair_proph : val :=
-    rec: "readPair" "l" :=
-      let: "xv1"    := readX "l"           in
-      let: "proph"  := NewProph            in
-      let: "y"      := readY "l"           in
-      let: "xv2"    := readX "l"           in
-      let: "v2"     := Snd "xv2"           in
-      let: "v_eq"   := Snd "xv1" = "v2"    in
-      resolve_proph: "proph" to: "v_eq" ;;
-      if: "v_eq"
-        then (Fst "xv1", "y")
-      else "readPair" "l".
-
   Variable N: namespace.
 
   Definition gmap_to_UR T : timestampUR := to_agree <$> T.
 
-  Definition pair_inv γ1 γ2 l1 l2 : iProp Σ :=
-    (∃ q (l1':loc) (T : gmap Z val) x y (t : Z),
+  Definition pair_inv γ1 γ2 l1 : iProp Σ :=
+    (∃ q (l1':loc) (T : gmap Z val) x (t : Z),
       (* we add the q to make the l1' map fractional. that way,
          we can take a fraction of the l1' map out of the invariant
          and do a case analysis on whether the pointer is the same
          throughout invariant openings *)
-      l1 ↦ #l1' ∗ l1' ↦{q} (x, #t) ∗ l2 ↦ y ∗
-         own γ1 (● Excl' (x, y)) ∗ own γ2 (● gmap_to_UR T) ∗
+      l1 ↦ #l1' ∗ l1' ↦{q} (x, #t) ∗
+         own γ1 (● Excl' x) ∗ own γ2 (● gmap_to_UR T) ∗
          ⌜T !! t = Some x⌝ ∗
          ⌜forall (t' : Z), t' ∈ dom (gset Z) T → (t' <= t)%Z⌝)%I.
 
-  Definition is_pair (γs: gname * gname) (p : val) :=
-    (∃ (l1 l2 : loc), ⌜p = (#l1, #l2)%V⌝ ∗ inv N (pair_inv γs.1 γs.2 l1 l2))%I.
+  Definition is_pair (γs: gname * gname * loc) (p : val) :=
+    (∃ (l1 : loc), ⌜p = (#l1, #γs.2)%V⌝ ∗ inv N (pair_inv γs.1.1 γs.1.2 l1))%I.
 
   Global Instance is_pair_persistent γs p : Persistent (is_pair γs p) := _.
 
-  Definition pair_content (γs : gname * gname) (a : val * val) :=
-    (own γs.1 (◯ Excl' a))%I.
+  Definition pair_content (γs : gname * gname * loc) (a : val * val) :=
+    (own γs.1.1 (◯ Excl' a.1) ∗ γs.2 ↦ a.2)%I.
 
   Global Instance pair_content_timeless γs a : Timeless (pair_content γs a) := _.
 
   Lemma pair_content_exclusive γs a1 a2 :
     pair_content γs a1 -∗ pair_content γs a2 -∗ False.
   Proof.
-    iIntros "H1 H2". iDestruct (own_valid_2 with "H1 H2") as %[].
+    iIntros "[H1 _] [H2 _]". iDestruct (own_valid_2 with "H1 H2") as %[].
   Qed.
 
   Definition new_timestamp t v : gmap Z val := {[ t := v ]}.
@@ -152,14 +154,14 @@ Section atomic_snapshot.
         newPair (v1, v2)%V
       {{{ γs p, RET p; is_pair γs p ∗ pair_content γs (v1, v2) }}}.
   Proof.
-    iIntros (Φ _) "Hp". rewrite /newPair. wp_lam.
+    iIntros (Φ _) "Hx". rewrite /newPair. wp_lam.
     repeat (wp_proj; wp_let).
     iApply wp_fupd.
+    wp_alloc ly as "Hly".
     wp_alloc lx' as "Hlx'".
     wp_alloc lx as "Hlx".
-    wp_alloc ly as "Hly".
-    set (Excl' (v1, v2)) as p.
-    iMod (own_alloc (● p ⋅ ◯ p)) as (γ1) "[Hp⚫ Hp◯]". {
+    set (Excl' v1) as p.
+    iMod (own_alloc (● p ⋅ ◯ p)) as (γ1) "[Hx⚫ Hx◯]". {
       rewrite /p. apply auth_both_valid. split; done.
     }
     set (new_timestamp 0 v1) as t.
@@ -167,14 +169,14 @@ Section atomic_snapshot.
       rewrite /t /new_timestamp. apply auth_both_valid.
       split; first done. rewrite /gmap_to_UR map_fmap_singleton. apply singleton_valid. done.
     }
-    wp_pures. iApply ("Hp" $! (γ1, γ2)).
-    iMod (inv_alloc N _ (pair_inv γ1 γ2 _ _) with "[-Hp◯ Ht◯]") as "#Hinv". {
-      iNext. rewrite /pair_inv. iExists _, _, _, _, _. iExists 0. iFrame.
+    wp_pures. iApply ("Hx" $! (γ1, γ2, ly)).
+    iMod (inv_alloc N _ (pair_inv γ1 γ2 _) with "[-Hx◯ Ht◯ Hly]") as "#Hinv". {
+      iNext. rewrite /pair_inv. iExists _, _, _, _, 0. iFrame.
       iPureIntro. split; first done. intros ?. subst t. rewrite /new_timestamp dom_singleton.
       rewrite elem_of_singleton. lia.
     }
-    iModIntro. iSplitR. rewrite /is_pair. repeat (iExists _). iSplitL; eauto.
-    rewrite /pair_content. rewrite /p. iApply "Hp◯".
+    iModIntro. rewrite /is_pair /pair_content. iFrame. iExists _.
+    iSplitL; first done. done.
   Qed.
 
  Lemma excl_update γ n' n m :
@@ -239,20 +241,15 @@ Section atomic_snapshot.
         @ ⊤∖↑N
       <<< pair_content γ (x, y2), RET #() >>>.
   Proof.
-    iIntros "Hp". iIntros (Φ) "AU".
-    iDestruct "Hp" as (l1 l2 ->) "#Hinv". wp_pures.
+    iIntros "Hx". iIntros (Φ) "AU".
+    iDestruct "Hx" as (l1 ->) "#Hinv". wp_pures.
     wp_lam. wp_pures.
     iApply wp_fupd.
-    iInv N as (q l1' T x) "Hinvp".
-    iDestruct "Hinvp" as (y v') "[Hl1 [Hl1' [Hl2 [Hp⚫ Htime]]]]".
+    iMod "AU" as (xv yv) "[[Hx Hy] [_ Hclose]]".
     wp_store.
-    iMod "AU" as (xv yv) "[Hpair [_ Hclose]]".
-    rewrite /pair_content.
-    iDestruct (excl_sync with "Hp⚫ Hpair") as %[= -> ->].
-    iMod (excl_update _ (x, y2) with "Hp⚫ Hpair") as "[Hp⚫ Hp◯]".
-    iMod ("Hclose" with "Hp◯") as "HΦ".
-    iModIntro. iSplitR "HΦ"; last done.
-    iNext. unfold pair_inv. eauto 7 with iFrame.
+    iMod ("Hclose" with "[Hx Hy]") as "HΦ".
+    { rewrite /pair_content. iFrame. }
+    eauto.
   Qed.
 
   Lemma writeX_spec γ (x2: val) p :
@@ -262,12 +259,11 @@ Section atomic_snapshot.
         @ ⊤∖↑N
       <<< pair_content γ (x2, y), RET #() >>>.
   Proof.
-    iIntros "Hp". iIntros (Φ) "AU". iLöb as "IH".
-    iDestruct "Hp" as (l1 l2 ->) "#Hinv". wp_pures. wp_lam. wp_pures.
+    iIntros "Hx". iIntros (Φ) "AU". iLöb as "IH".
+    iDestruct "Hx" as (l1 ->) "#Hinv". wp_pures. wp_lam. wp_pures.
     (* first read *)
     (* open invariant *)
-    wp_bind (!_)%E. iInv N as (q l1' T x) "Hinvp".
-      iDestruct "Hinvp" as (y v') "[Hl1 [Hl1' [Hl2 [Hp⚫ Htime]]]]".
+    wp_bind (!_)%E. iInv N as (q l1' T x v') "[Hl1 [Hl1' [Hx⚫ Htime]]]".
       wp_load.
       iDestruct "Hl1'" as "[Hl1'frac1 Hl1'frac2]".
       iModIntro. iSplitR "AU Hl1'frac2".
@@ -279,19 +275,19 @@ Section atomic_snapshot.
     (* CAS *)
     wp_bind (CAS _ _ _)%E.
     (* open invariant *)
-    iInv N as (q' l1'' T x') ">Hinvp".
-    iDestruct  "Hinvp" as (y' v'') "[Hl1 [Hl1'' [Hl2 [Hp⚫ [Ht● Ht]]]]]".
+    iInv N as (q' l1'' T x' v'') ">[Hl1 [Hl1'' [Hx⚫ [Ht● Ht]]]]".
     iDestruct "Ht" as %[Ht Hvt].
     destruct (decide (l1'' = l1')) as [-> | Hn].
     - wp_cas_suc.
       iDestruct (mapsto_agree with "Hl1'frac2 Hl1''") as %[= -> ->]. iClear "Hl1'frac2".
       (* open AU *)
-      iMod "AU" as (xv yv) "[Hpair [_ Hclose]]".
+      iMod "AU" as (xv yv) "[[Hx Hy] [_ Hclose]]".
         (* update pair ghost state to (x2, y') *)
-        iDestruct (excl_sync with "Hp⚫ Hpair") as %[= -> ->].
-        iMod (excl_update _ (x2, y') with "Hp⚫ Hpair") as "[Hp⚫ Hp◯]".
+        iDestruct (excl_sync with "Hx⚫ Hx") as %[= ->].
+        iMod (excl_update _ x2 with "Hx⚫ Hx") as "[Hx⚫ Hx◯]".
         (* close AU *)
-        iMod ("Hclose" with "Hp◯") as "HΦ".
+        iMod ("Hclose" with "[Hx◯ Hy]") as "HΦ".
+        { rewrite /pair_content. iFrame. }
       (* update timestamp *)
       iMod (timestamp_update _ T (v'' + 1)%Z x2 with "[Ht●]") as "Ht".
       { eapply (not_elem_of_dom (D:=gset Z) T). intros Hd. specialize (Hvt _ Hd). omega. }
@@ -300,7 +296,7 @@ Section atomic_snapshot.
       iModIntro. iSplitR "HΦ".
       + iNext. rewrite /pair_inv.
         set (<[ v'' + 1 := x2]> T) as T'.
-        iExists 1%Qp, l1'new, T', x2, y', (v'' + 1).
+        iExists 1%Qp, l1'new, T', x2, (v'' + 1).
         iFrame.
         iPureIntro. split.
         * apply: lookup_insert.
@@ -324,19 +320,15 @@ Section atomic_snapshot.
       @ ⊤∖↑N
     <<< pair_content γ (v1, v2), RET v2 >>>.
   Proof.
-    iIntros "Hp". iIntros (Φ) "AU".
-    iDestruct "Hp" as (l1 l2 ->) "#Hinv".
+    iIntros "Hx". iIntros (Φ) "AU".
+    iDestruct "Hx" as (l1 ->) "#Hinv".
     repeat (wp_lam; wp_proj). wp_let.
     iApply wp_fupd.
-    iInv N as (q l1' T x) "Hinvp".
-    iDestruct "Hinvp" as (y v') "[Hl1 [Hl1' [Hl2 [Hp⚫ Htime]]]]".
+    iMod "AU" as (xv yv) "[[Hx Hy] [_ Hclose]]".
     wp_load.
-    iMod "AU" as (xv yv) "[Hpair [_ Hclose]]".
     rewrite /pair_content.
-    iDestruct (excl_sync with "Hp⚫ Hpair") as %[= -> ->].
-    iMod ("Hclose" with "Hpair") as "HΦ".
-    iModIntro. iSplitR "HΦ"; last done.
-    iNext. unfold pair_inv. eauto 7 with iFrame.
+    iMod ("Hclose" with "[$Hx $Hy]") as "HΦ".
+    iModIntro. done.
   Qed.
 
   Lemma readX_spec γ p :
@@ -346,23 +338,22 @@ Section atomic_snapshot.
       @ ⊤∖↑N
     <<< ∃ (t: Z), pair_content γ (v1, v2), RET (v1, #t) >>>.
   Proof.
-    iIntros "Hp". iIntros (Φ) "AU".
-    iDestruct "Hp" as (l1 l2 ->) "#Hinv".
+    iIntros "Hx". iIntros (Φ) "AU".
+    iDestruct "Hx" as (l1 ->) "#Hinv".
     repeat (wp_lam; wp_proj). wp_let. wp_bind (! #l1)%E.
     (* open invariant for 1st read *)
-    iInv N as (q l1' T x) ">Hinvp".
-      iDestruct "Hinvp" as (y v') "[Hl1 [Hl1' [Hl2 [Hp⚫ Htime]]]]".
+    iInv N as (q l1' T x v') ">[Hl1 [Hl1' [Hx⚫ Htime]]]".
       wp_load.
       iDestruct "Hl1'" as "[Hl1' Hl1'frac]".
-      iMod "AU" as (xv yv) "[Hpair [_ Hclose]]".
-      iDestruct (excl_sync with "Hp⚫ Hpair") as %[= -> ->].
-      iMod ("Hclose" with "Hpair") as "HΦ".
+      iMod "AU" as (xv yv) "[[Hx Hy] [_ Hclose]]".
+      iDestruct (excl_sync with "Hx⚫ Hx") as %[= ->].
+      iMod ("Hclose" with "[Hx Hy]") as "HΦ".
+      { rewrite /pair_content. iFrame. }
       (* close invariant *)
       iModIntro. iSplitR "HΦ Hl1'". {
         iNext. unfold pair_inv. eauto 7 with iFrame.
       }
-    iApply wp_fupd. clear T y.
-    wp_load. eauto.
+    iApply wp_fupd. wp_load. eauto.
   Qed.
 
   Definition prophecy_to_bool (v : list (val * val)) : bool :=
@@ -378,20 +369,20 @@ Section atomic_snapshot.
        @ ⊤∖↑N
     <<< pair_content γ (v1, v2), RET (v1, v2) >>>.
   Proof.
-    iIntros "Hp". iIntros (Φ) "AU". iLöb as "IH".
+    iIntros "Hx". iIntros (Φ) "AU". iLöb as "IH".
     wp_pures.
     (* ************ 1st readX ********** *)
-    iDestruct "Hp" as (l1 l2 ->) "#Hinv". repeat (wp_lam; wp_pures).
+    iDestruct "Hx" as (l1 ->) "#Hinv". repeat (wp_lam; wp_pures).
     wp_bind (! #l1)%E.
     (* open invariant for 1st read *)
-    iInv N as (q_x1 l1' T_x x1) ">Hinvp".
-      iDestruct "Hinvp" as (y_x1 v_x1) "[Hl1 [Hl1' [Hl2 [Hp⚫ [Ht_x Htime_x]]]]]".
+    iInv N as (q_x1 l1' T_x x1 v_x1) ">[Hl1 [Hl1' [Hx⚫ [Ht_x Htime_x]]]]".
       iDestruct "Htime_x" as %[Hlookup_x Hdom_x].
       wp_load.
       iDestruct "Hl1'" as "[Hl1' Hl1'frac]".
-      iMod "AU" as (xv yv) "[Hpair [Hclose _]]".
-      iDestruct (excl_sync with "Hp⚫ Hpair") as %[= -> ->].
-      iMod ("Hclose" with "Hpair") as "AU".
+      iMod "AU" as (xv yv) "[[Hx Hy] [Hclose _]]".
+      iDestruct (excl_sync with "Hx⚫ Hx") as %[= ->].
+      iMod ("Hclose" with "[Hx Hy]") as "AU".
+      { rewrite /pair_content. iFrame. }
       (* duplicate timestamp T_x1 *)
       iMod (timestamp_dupl with "Ht_x") as "[Ht_x1⚫ Ht_x1◯]".
       (* close invariant *)
@@ -405,24 +396,24 @@ Section atomic_snapshot.
     wp_let.
     (* ************ readY ********** *)
     repeat (wp_lam; wp_pures). wp_bind (!_)%E.
-    iInv N as (q_y l1'_y T_y x_y) ">Hinvp".
-    iDestruct "Hinvp" as (y_y v_y) "[Hl1 [Hl1'_y [Hl2 [Hp⚫ [Ht_y Htime_y]]]]]".
+    iInv N as (q_y l1'_y T_y x_y v_y) ">[Hl1 [Hl1'_y [Hx⚫ [Ht_y Htime_y]]]]".
     iDestruct "Htime_y" as %[Hlookup_y Hdom_y].
-    wp_load.
     (* linearization point *)
-    iMod "AU" as (xv yv) "[Hpair Hclose]".
+    clear yv.
+    iMod "AU" as (xv yv) "[[Hx Hy] Hclose]".
+    wp_load.
     rewrite /pair_content.
-    iDestruct (excl_sync with "Hp⚫ Hpair") as %[= -> ->].
+    iDestruct (excl_sync with "Hx⚫ Hx") as %[= ->].
     destruct (prophecy_to_bool proph_val) eqn:Hproph.
     - (* prophecy value is predicting that timestamp has not changed, so we commit *)
       (* committing AU *)
-      iMod ("Hclose" with "Hpair") as "HΦ".
+      iMod ("Hclose" with "[$Hx $Hy]") as "HΦ".
       (* duplicate timestamp T_y *)
       iMod (timestamp_dupl with "Ht_y") as "[Ht_y● Ht_y◯]".
       (* show that T_x <= T_y *)
       iDestruct (timestamp_sub with "[Ht_y● Ht_x1◯]") as "#Hs"; first by iFrame.
       iDestruct "Hs" as %Hs.
-      iModIntro.
+      iModIntro. iModIntro.
       (* closing invariant *)
       iSplitR "HΦ Hl1' Ht_x1◯ Ht_y◯ Hpr".
       { iNext. unfold pair_inv. eauto 10 with iFrame. }
@@ -430,8 +421,7 @@ Section atomic_snapshot.
       (* ************ 2nd readX ********** *)
       repeat (wp_lam; wp_pures). wp_bind (! #l1)%E.
       (* open invariant *)
-      iInv N as (q_x2 l1'_x2 T_x2 x2) ">Hinvp".
-      iDestruct "Hinvp" as (y_x2 v_x2) "[Hl1 [Hl1'_x2 [Hl2 [Hp⚫ [Ht_x2 Htime_x2]]]]]".
+      iInv N as (q_x2 l1'_x2 T_x2 x2 v_x2) ">[Hl1 [Hl1'_x2 [Hx⚫ [Ht_x2 Htime_x2]]]]".
       iDestruct "Htime_x2" as %[Hlookup_x2 Hdom_x2].
       iDestruct "Hl1'_x2" as "[Hl1'_x2 Hl1'_x2_frag]".
       wp_load.
@@ -461,8 +451,8 @@ Section atomic_snapshot.
         }
         done.
       + inversion Hproph.
-    - iDestruct "Hclose" as "[Hclose _]". iMod ("Hclose" with "Hpair") as "AU".
-      iModIntro.
+    - iDestruct "Hclose" as "[Hclose _]". iMod ("Hclose" with "[$Hx $Hy]") as "AU".
+      iModIntro. iModIntro.
       (* closing invariant *)
       iSplitR "AU Hpr".
       { iNext. unfold pair_inv. eauto 10 with iFrame. }
@@ -470,8 +460,7 @@ Section atomic_snapshot.
       (* ************ 2nd readX ********** *)
       repeat (wp_lam; wp_proj). wp_let. wp_bind (! #l1)%E.
       (* open invariant *)
-      iInv N as (q_x2 l1'_x2 T_x2 x2) ">Hinvp".
-      iDestruct "Hinvp" as (y_x2 v_x2) "[Hl1 [Hl1'_x2 [Hl2 [Hp⚫ [Ht_x2 Htime_x2]]]]]".
+      iInv N as (q_x2 l1'_x2 T_x2 x2 v_x2) "[Hl1 [Hl1'_x2 [Hx⚫ [Ht_x2 Htime_x2]]]]".
       iDestruct "Hl1'_x2" as "[Hl1'_x2 Hl1'_x2_frag]".
       wp_load.
       iModIntro. iSplitR "AU Hl1'_x2_frag Hpr". {
